\chapter{Abstract}



\section{Proof of the Graph Method for Transport Equations.\label{sec:AbsGraphmethod}}



\section{Initial DQD-Majorana Hamiltonian.\label{chap:Double-Dot-Majorana-Hamiltonian.}}

$H_{N_{\uparrow}=0,P_{\downarrow}=-1}:$
\[
\begin{array}{c}
\vert\downarrow,\downarrow,\downarrow\rangle\rightarrow\\
\vert0,0,\downarrow\rangle\rightarrow\\
\vert0,\downarrow,0\rangle\rightarrow\\
\vert\downarrow,0,0\rangle\rightarrow
\end{array}\left[\begin{array}{cccc}
\epsilon_{d}^{+}+\frac{U^{+}}{2}-2h+\epsilon_{m} & 0 & -\tilde{t}_{+1} & \tilde{t}_{+2}\\
0 & \frac{U^{+}}{2}+\epsilon_{m} & \tilde{t}_{-2}^{*} & \tilde{t}_{-1}^{*}\\
-\tilde{t}_{+1}^{*} & \tilde{t}_{-2} & \epsilon_{d_{2}}+\frac{U^{+}}{2}-h-\epsilon_{m} & t\\
\tilde{t}_{+2}^{*} & \tilde{t}_{-1} & t^{*} & \epsilon_{d_{1}}+\frac{U^{+}}{2}-h-\epsilon_{m}
\end{array}\right]
\]


$H_{N_{\uparrow}=0,P_{\downarrow}=1}:$
\[
\begin{array}{c}
\vert0,0,0\rangle\rightarrow\\
\vert\downarrow,\downarrow,0\rangle\rightarrow\\
\vert\downarrow,0,\downarrow\rangle\rightarrow\\
\vert0,\downarrow,\downarrow\rangle\rightarrow
\end{array}\left[\begin{array}{cccc}
\frac{U^{+}}{2}-\epsilon_{m} & 0 & \tilde{t}_{+1} & \tilde{t}_{+2}\\
0 & \epsilon_{d}^{+}+\frac{U^{+}}{2}-2h-\epsilon_{m} & \tilde{t}_{-2}^{*} & -\tilde{t}_{-1}^{*}\\
\tilde{t}_{+1}^{*} & \tilde{t}_{-2} & \epsilon_{d_{1}}+\frac{U^{+}}{2}-h+\epsilon_{m} & t\\
\tilde{t}_{+2}^{*} & -\tilde{t}_{-1} & t^{*} & \epsilon_{d_{2}}+\frac{U^{+}}{2}-h+\epsilon_{m}
\end{array}\right]
\]


$H_{N_{\uparrow}=2,P_{\downarrow}=-1}:$
\[
\begin{array}{c}
\vert\uparrow\!\downarrow,\uparrow\!\downarrow,\downarrow\rangle\rightarrow\\
\vert\uparrow,\uparrow,\downarrow\rangle\rightarrow\\
\vert\uparrow,\uparrow\!\downarrow,0\rangle\rightarrow\\
\vert\uparrow\!\downarrow,\uparrow,0\rangle\rightarrow
\end{array}\left[\begin{array}{cccc}
2\epsilon_{d}^{+}+\frac{3U^{+}}{2}+\epsilon_{m} & 0 & \tilde{t}_{+1} & \tilde{t}_{+2}\\
0 & \epsilon_{d}^{+}+\frac{U^{+}}{2}+2h+\epsilon_{m} & \tilde{t}_{-2}^{*} & -\tilde{t}_{-1}^{*}\\
\tilde{t}_{+1}^{*} & \tilde{t}_{-2} & f(d_{1},d_{2})+h-\epsilon_{m} & -t\\
\tilde{t}_{+2}^{*} & -\tilde{t}_{-1} & -t^{*} & f(d_{2},d_{1})+h-\epsilon_{m}
\end{array}\right]
\]


with $f(d_{i},d_{j})=\epsilon_{d_{i}}+\frac{U_{i}}{2}+2\epsilon_{d_{j}}+\frac{3U_{j}}{2}.$

$H_{N_{\uparrow}=2,P_{\downarrow}=1}:$
\[
\begin{array}{c}
\vert\uparrow,\uparrow,0\rangle\rightarrow\\
\vert\uparrow\!\downarrow,\uparrow\!\downarrow,0\rangle\rightarrow\\
\vert\uparrow\!\downarrow,\uparrow,\downarrow\rangle\rightarrow\\
\vert\uparrow,\uparrow\!\downarrow,\downarrow\rangle\rightarrow
\end{array}\left[\begin{array}{cccc}
\epsilon_{d}^{+}+\frac{U^{+}}{2}+2h-\epsilon_{m} & 0 & -\tilde{t}_{+1} & \tilde{t}_{+2}\\
0 & 2\epsilon_{d}^{+}+\frac{3U^{+}}{2}-\epsilon_{m} & \tilde{t}_{-2}^{*} & \tilde{t}_{-1}^{*}\\
-\tilde{t}_{+1}^{*} & \tilde{t}_{-2} & f(d_{2},d_{1})+h+\epsilon_{m} & -t\\
\tilde{t}_{+2}^{*} & \tilde{t}_{-1} & -t^{*} & f(d_{1},d_{2})+h+\epsilon_{m}
\end{array}\right]
\]
